GF2.v
@@ -1,0 +1,139 @@
+Require Import VST.floyd.functional_base.
+Require Import Coq.setoid_ring.Ring_theory.
+Require Import Coq.setoid_ring.Field_theory.
+(** The field GF(2), represented as bits *)
+
+Inductive bit :=
+  | Zero
+  | One.
+
+Notation "0" := Zero.
+Notation "1" := One.
+
+Ltac solve_bit :=
+  repeat(match goal with
+  | [x : bit |- _ ] => destruct x; try reflexivity
+  end).
+
+Instance bit_default : Inhabitant bit.
+apply Zero.
+Defined.
+
+Definition bit_add (b1 b2 : bit) :=
+  match (b1, b2) with
+  | (1, 1) => 0
+  | (0, 0) => 0
+  | (_, _) => 1
+  end.
+
+Lemma bit_add_comm: forall b1 b2,
+  bit_add b1 b2 = bit_add b2 b1.
+Proof.
+  intros. solve_bit.
+Qed.
+
+Lemma bit_add_assoc : forall b1 b2 b3,
+  bit_add (bit_add b1 b2) b3 = bit_add b1 (bit_add b2 b3).
+Proof.
+  intros; solve_bit.
+Qed.
+
+Lemma bit_add_0_l: forall b,
+  bit_add 0 b = b.
+Proof.
+  intros; solve_bit. 
+Qed.
+
+Lemma bit_add_0_r: forall b,
+  bit_add b 0 = b.
+Proof.
+  intros; solve_bit.
+Qed.
+
+Definition eq_bit (b1 b2 : bit) :=
+  match (b1, b2) with
+  | (1, 1) => true
+  | (0, 0) => true
+  | (_, _) => false
+  end.
+
+Lemma eq_bit_eq: forall b1 b2,
+  eq_bit b1 b2 = true <-> b1 = b2.
+Proof.
+  intros; split; intros; solve_bit; inversion H.
+Qed.
+
+Definition bit_mult (b1 b2 : bit) : bit :=
+  match b1, b2 with
+  | 1, 1 => 1
+  | _, _ => 0
+  end.
+
+Lemma bit_mult_comm: forall b1 b2,
+  bit_mult b1 b2 = bit_mult b2 b1.
+Proof.
+  intros; solve_bit. 
+Qed.
+
+Lemma bit_mult_assoc: forall b1 b2 b3,
+  bit_mult (bit_mult b1 b2) b3 = bit_mult b1 (bit_mult b2 b3).
+Proof.
+  intros; solve_bit. 
+Qed.
+
+Lemma bit_mult_0_l: forall b,
+  bit_mult 0 b = 0.
+Proof.
+  intros; solve_bit. 
+Qed.
+
+Lemma bit_mult_0_r: forall b,
+  bit_mult b 0 = 0.
+Proof.
+  intros; solve_bit. 
+Qed.
+
+Lemma bit_mult_1_l:
+  forall b,
+  bit_mult 1 b = b.
+Proof.
+  intros; solve_bit.
+Qed.
+
+Lemma bit_mult_1_r:
+  forall b,
+  bit_mult b 1 = b.
+Proof.
+  intros; solve_bit. 
+Qed.
+
+Lemma bit_distr: forall b1 b2 b3,
+  bit_mult (bit_add b1 b2) b3  = bit_add (bit_mult b1 b3) (bit_mult b2 b3).
+Proof.
+  intros; solve_bit. 
+Qed.
+
+Definition bit_ring: @ring_theory bit 0 1 bit_add bit_mult bit_add id eq.
+Proof.
+apply mk_rt.
+- apply bit_add_0_l.
+- apply bit_add_comm.
+- intros; symmetry; apply bit_add_assoc.
+- apply bit_mult_1_l.
+- apply bit_mult_comm.
+- intros; symmetry; apply bit_mult_assoc.
+- apply bit_distr.
+- reflexivity.
+- intros. solve_bit.
+Defined.
+
+Definition bit_field: @field_theory bit 0 1 bit_add bit_mult bit_add id bit_mult id eq.
+Proof.
+apply mk_field.
+- apply bit_ring.
+- intro. inversion H.
+- intros. solve_bit.
+- intros. solve_bit. contradiction.
+Defined.
+
+
