Helper.v
@@ -1,0 +1,119 @@
+Require Import Coq.Lists.List.
+Require Import Coq.Bool.Bool.
+Require Import VST.floyd.functional_base.
+(** Contains definitions and lemmas that are useful more generally *)
+
+Definition null {A} (l: list A) :=
+  match l with
+  | nil => true
+  | _ => false
+  end.
+
+(* function (from Haskell) to remove all values from end of list that satisfy a predicate. *)
+Definition dropWhileEnd {A} (p: A -> bool)(l: list A)  : list A :=
+  fold_right (fun x acc => if (null acc) && (p x) then nil else x :: acc) nil l.
+
+Lemma dropWhileEnd_nil: forall {A} p (l: list A),
+  dropWhileEnd p l = nil <-> forall x, In x l -> p x = true.
+Proof.
+  intros. induction l; split; intros.
+  - inversion H0.
+  - reflexivity.
+  - simpl in H. destruct (null (dropWhileEnd p l)) eqn : N. simpl in H. destruct (p a) eqn : P.
+    + destruct H0. subst. assumption. apply IHl. destruct (dropWhileEnd p l). reflexivity. inversion N. assumption.
+    + inversion H.
+    + simpl in H. inversion H.
+  - simpl. destruct ((dropWhileEnd p l)) eqn : D. simpl. assert (p a = true). apply H. left. reflexivity.
+    rewrite H0. reflexivity. assert (a0 :: l0 = nil). apply IHl. intros. apply H. right. assumption.
+    inversion H0.
+Qed. 
+
+Lemma dropWhileEnd_spec: forall {A} p (l: list A) (y: A) res,
+  dropWhileEnd p l = res <->
+  (exists l1, l = res ++ l1 /\ forall x, In x l1 -> p x = true) /\
+  (res <> nil -> p (last res y) = false).
+Proof.
+  intros. split; intros; subst. induction l; simpl; split.
+  - exists nil. auto.
+  - intros. contradiction.
+  - destruct IHl. destruct (dropWhileEnd p l) eqn : L.
+    + simpl. destruct (p a) eqn : P.
+      * exists (a :: l). simpl. split. reflexivity. intros. destruct H1. subst. assumption.
+        destruct H. destruct H. simpl in H; subst. apply H2. assumption.
+      * exists l. simpl. split. reflexivity. destruct H. destruct H. simpl in H; subst. apply H1.
+    + simpl. destruct H as [l1]. destruct H. subst. exists l1. split. reflexivity. apply H1.
+  - destruct IHl. destruct (dropWhileEnd p l) eqn : L; simpl.
+    + destruct (p a) eqn : P.
+      * intros. contradiction.
+      * intros. simpl. assumption.
+    + intros. simpl in H0. apply H0. intro. inversion H2.
+  - destruct H. destruct H as [l1]. destruct H. rewrite H. unfold dropWhileEnd. rewrite fold_right_app.
+    assert ((fold_right (fun (x : A) (acc : list A) => if null acc && p x then nil else x :: acc) nil l1) =
+    dropWhileEnd p l1). unfold dropWhileEnd. reflexivity. rewrite H2; clear H2.
+    assert (dropWhileEnd p l1 = nil). apply dropWhileEnd_nil. apply H1. rewrite H2.
+    assert (fold_right (fun (x : A) (acc : list A) => if null acc && p x then nil else x :: acc) nil res
+    = dropWhileEnd p res) by reflexivity. rewrite H3; clear H3.
+    clear H2. clear H1. clear H. induction res.
+    + reflexivity.
+    + simpl. destruct (dropWhileEnd p res) eqn : D.
+      * simpl. destruct (p a) eqn : P. simpl in H0. destruct res.
+        rewrite H0 in P. inversion P. intro. inversion H.
+        assert (nil = a0 :: res). apply IHres. intros. apply H0. intro. inversion H1. inversion H.
+        destruct res. reflexivity. rewrite IHres. reflexivity. intros. simpl. simpl in H0. apply H0.
+        intro. inversion H1.
+      * simpl. destruct res. simpl in IHres. rewrite IHres. reflexivity. intros. contradiction.
+        rewrite IHres. reflexivity. intros. simpl. simpl in H0. apply H0. intro. inversion H1; simpl in IHres.
+Qed.
+
+Lemma Znth_nil: forall {A} `{d: Inhabitant A} z,
+  Znth z (@nil A) = d.
+Proof.
+  intros. assert (z < 0 \/ z >= 0) by lia. destruct H.
+  - rewrite Znth_underflow; try lia. reflexivity.
+  - rewrite Znth_overflow. reflexivity. list_solve.
+Qed.
+
+Lemma Znth_last: forall {A} `{Inhabitant A} (l: list A) x,
+  l <> nil ->
+  Znth (Zlength l - 1) l = last l x.
+Proof.
+  intros A H l. induction l; intros.
+  - contradiction.
+  - destruct l.
+    + simpl. list_solve.
+    + simpl in IHl. simpl. rewrite <- IHl. list_solve. intro C; inversion C. 
+Qed.
+
+Lemma last_nonempty: forall {A} (l1: list A) l2 (x: A),
+  l2 <> nil ->
+  last (l1 ++ l2) x = last l2 x.
+Proof.
+  intros. induction l1.
+  - reflexivity.
+  - simpl. destruct ((l1 ++ l2)) eqn : L. 
+    destruct l1. destruct l2. contradiction. inversion L. inversion L. apply IHl1.
+Qed.
+
+Lemma last_in: forall {A} (l1: list A) (x: A),
+  l1 <> nil ->
+  In (last l1 x) l1.
+Proof.
+  intros. induction l1.
+  - contradiction.
+  - destruct l1. simpl. left. reflexivity. right. simpl in *. apply IHl1. intro C; inversion C. 
+Qed.  
+
+
+Lemma Znth_seq: forall start len z,
+  0 <= z < Z.of_nat len ->
+  Znth z (seq start len) = Z.to_nat (Z.of_nat start + z).
+Proof.
+  intros. rewrite <- nth_Znth. rewrite seq_nth. lia. lia. 
+  rewrite Zlength_correct. rewrite seq_length. lia.
+Qed. 
+
+Lemma Zlength_seq: forall start len,
+  Zlength (seq start len) = Z.of_nat len.
+Proof.
+  intros. rewrite Zlength_correct. rewrite seq_length. reflexivity.
+Qed. 
