PolyDiv.v
@@ -1,0 +1,190 @@
+Require Import VST.floyd.functional_base.
+Require Import GF2.
+Require Import Poly.
+(** * A verified, executable version of Euclidean division on polynomials over GF2 *)
+
+(** Monomials *)
+
+(*We provide a special shorthand for the monomial x^n, which will be useful in division*)
+
+Definition monomial (n: nat) :=
+  if Nat.eq_dec n 0%nat then (1 :: nil) else shift (1 :: nil) n.
+
+Lemma monomial_deg: forall n,
+  deg (monomial n) = Z.of_nat n.
+Proof.
+  intros. unfold monomial. if_tac. subst. simpl. reflexivity. rewrite deg_shift. unfold deg. list_solve.
+Qed.
+
+Lemma wf_monomial: forall n,
+  wf_poly (monomial n).
+Proof.
+  intros. unfold monomial. if_tac. unfold wf_poly; intros. reflexivity.
+  unfold shift. unfold wf_poly. intros. rewrite last_last. reflexivity.
+Qed.
+
+Lemma monomial_not_0: forall n,
+  monomial n <> nil.
+Proof.
+  intros. intro. unfold monomial in H. destruct (Nat.eq_dec n 0). inversion H.
+  unfold shift in H. destruct (list_repeat n 0); inversion H.
+Qed.
+
+(** Euclidean Division **)
+
+(*note: may want to make more efficient by shifting instead of add a monomial*)
+Program Fixpoint poly_div_aux (a b q r : poly) (Hb: wf_poly b) (Hr: wf_poly r) {measure (Z.to_nat (deg r + 1))} : 
+  {x: poly * poly | (0<= deg b) ->  wf_poly q ->
+   (deg (snd x) < deg b /\ wf_poly (fst x) /\ wf_poly (snd x) /\
+   (a = poly_add (poly_mult b q) r -> a = poly_add (poly_mult b (fst x)) (snd x)))}
+  :=
+  match b with
+  | nil => (nil, nil) (*cannot divide by zero *)
+  | (x :: t) =>
+  match (zlt (deg r) (deg b)) with
+  | left H => (q,r)
+  | right H' => let pow := monomial (Z.to_nat (deg r - deg b)) in
+                let q' := poly_add q pow in
+                let r' := poly_add r (poly_mult b pow) in
+                poly_div_aux a b q' r' Hb (wf_poly_add _ _)
+  end
+end.
+(*begin hide*)
+Next Obligation.
+lia.
+Defined.
+Next Obligation.
+destruct r.
+(*if r = 0 - contradiction*)
+simpl in H'. assert (Zlength (x :: t) > 0) by list_solve. lia.
+(*now handle case when r' = 0*)
+assert (forall l, deg l = -1 \/ 0 <= deg l). { intros. unfold deg; destruct l. left. reflexivity.
+right. list_solve. }
+remember (poly_add (b :: r) (poly_mult (x :: t) (monomial (Z.to_nat (deg (b :: r) - deg (x :: t)))))) as r'.
+specialize (H r'). destruct H.
+- destruct r'. simpl. list_solve. unfold deg in H. list_solve. 
+- (*now we can handle the usual case, and use the fact that polys of same degree result in a smaller poly when
+    multiplied together *)
+assert (deg (b :: r) = deg  (poly_mult (x :: t) (monomial (Z.to_nat (deg (b :: r) - deg (x :: t)))))). {
+rewrite poly_mult_deg. rewrite monomial_deg. lia. assumption. apply wf_monomial. simpl. 
+solve_neq. apply monomial_not_0. }
+assert ((deg (poly_add (b :: r) (poly_mult (x :: t) (monomial (Z.to_nat (deg (b :: r) - deg (x :: t)))))))
+  < (deg (b :: r))). {
+apply (poly_add_degree_same (b :: r) (poly_mult (x :: t) (monomial (Z.to_nat (deg (b :: r) - deg (x :: t)))))).
+- assumption.
+- apply wf_poly_mult. assumption. apply wf_monomial.
+- assumption.
+- simpl. list_solve. } 
+subst. list_solve.
+Defined.
+Next Obligation.
+destruct ((poly_div_aux a (x :: t) (poly_add q (monomial (Z.to_nat (deg r - deg (x :: t)))))
+           (poly_add r (poly_mult (x :: t) (monomial (Z.to_nat (deg r - deg (x :: t)))))) Hb
+           (wf_poly_add r (poly_mult (x :: t) (monomial (Z.to_nat (deg r - deg (x :: t))))))
+           (poly_div_aux_func_obligation_3 (x :: t) r Hb Hr poly_div_aux x t eq_refl H' Heq_anonymous))). simpl.
+(*in a more workable form - now to prove correctness - ie, that invariant is preserved*)
+destruct x0; simpl in *. 
+assert (wf_poly (poly_add q (monomial (Z.to_nat (deg r - (Zlength (x :: t) - 1)))))).
+apply wf_poly_add. specialize (a0 H H1). destruct a0. destruct H3. destruct H4. split.
+assumption. split. assumption. split. assumption. intros. apply H5. rewrite H6.
+remember (x :: t) as b.
+remember  (monomial (Z.to_nat (deg r - (Zlength b - 1)))) as pow.
+rewrite poly_mult_distr_l.
+symmetry. rewrite poly_add_assoc. f_equal. rewrite poly_add_comm.
+rewrite poly_add_assoc. rewrite poly_add_inv. rewrite poly_add_comm. apply poly_add_id. apply Hr.
+assumption. assumption. subst. apply wf_monomial.
+Defined.
+(*end hide*)
+
+Definition poly_div a b (Ha: wf_poly a) (Hb : wf_poly b) : poly * poly :=
+  proj1_sig (poly_div_aux a b nil a Hb Ha).
+
+(*begin hide*)
+
+Definition testa := (1 :: 1 :: 0 :: 1 :: nil).
+Lemma wf_a : wf_poly testa.
+Proof.
+unfold wf_poly. unfold testa. simpl. intros. reflexivity.
+Qed.
+
+Definition testb := (1 :: 1 :: nil).
+Lemma wf_b : wf_poly testb.
+Proof.
+  unfold wf_poly. unfold testb. simpl. reflexivity.
+Qed.
+
+Eval compute in (poly_add(poly_mult (0 :: 1 :: 1 :: nil) (1 :: 1 :: nil)) (1 :: nil)).
+Eval compute in ( poly_div testa testb wf_a wf_b  ).
+(*it works!*)
+(*end hide*)
+Section DivFacts.
+
+Lemma remainder_unique: forall a b q1 r1 q2 r2,
+  wf_poly a ->
+  wf_poly b ->
+  wf_poly q1 ->
+  wf_poly r1 ->
+  wf_poly q2 ->
+  wf_poly r2 ->
+  b <> nil ->
+  deg r1 < deg b ->
+  deg r2 < deg b ->
+  a = poly_add (poly_mult q1 b) r1 ->
+  a = poly_add (poly_mult q2 b) r2 ->
+  q1 = q2 /\ r1 = r2.
+Proof.
+  intros. subst. rewrite poly_add_comm in H9. rewrite poly_add_cancel_1 in H9. symmetry in H9.
+  rewrite <- poly_add_assoc in H9.
+  rewrite poly_add_cancel_1 in H9.
+  assert (deg (poly_add r2 r1) = deg (poly_add (poly_mult q1 b) (poly_mult q2 b))). rewrite H9; reflexivity.
+  pose proof (poly_add_degree_max r2 r1).
+  rewrite <- poly_mult_distr_r in H8.
+  destruct (poly_add q1 q2) eqn : P. all: try assumption. all: try (apply wf_poly_add).
+  - rewrite poly_add_inv_iff in P; try assumption. subst. 
+    rewrite poly_mult_0_l in H8. simpl in H8.
+    destruct (poly_add r2 r1) eqn : R. rewrite poly_add_inv_iff in R; try assumption. auto.
+    simpl in H8. list_solve.
+  - rewrite <- P in H8. rewrite poly_mult_deg in H8.
+    assert (deg (poly_add q1 q2) < 0) by lia.
+    assert (poly_add q1 q2 = nil). destruct (poly_add q1 q2). reflexivity. simpl in H11.
+    list_solve. rewrite poly_add_inv_iff in H12. subst.
+    rewrite poly_add_inv in H9. symmetry in H9. rewrite poly_add_inv_iff in H9. subst. auto.
+    all: try assumption. all: try(apply wf_poly_add). intro. rewrite P in H11. inversion H11.
+Qed.
+
+Lemma poly_div_wf: forall a b q r (Ha: wf_poly a) (Hb: wf_poly b),
+  b <> nil ->
+  poly_div a b Ha Hb = (q,r) ->
+  wf_poly q /\ wf_poly r.
+Proof.
+  intros. unfold poly_div in H0. destruct  (poly_div_aux a b nil a Hb Ha).
+  simpl in H0. destruct x; subst. simpl in a0. inversion H0; subst. split. apply a0.
+  unfold deg. destruct b. contradiction. list_solve. apply wf_poly_nil.
+  apply a0. destruct b; simpl. contradiction. list_solve. apply wf_poly_nil.
+Qed. 
+  
+ 
+Lemma poly_div_correct: forall a b q r (Ha: wf_poly a) (Hb : wf_poly b),
+  wf_poly q ->
+  wf_poly r ->
+  b <> nil ->
+  deg r < deg b ->
+  poly_div a b Ha Hb = (q,r) <-> a = poly_add (poly_mult q b) r.
+Proof.
+  intros. split; intros.
+  - unfold poly_div in H3. destruct (poly_div_aux a b nil a Hb Ha). simpl in H3.
+    destruct x; inversion H3; subst; simpl in *. clear H3.
+    assert (deg r < deg b /\ wf_poly q /\ wf_poly r /\ (a = poly_add nil a -> a = poly_add (poly_mult b q) r)).
+    apply a0. destruct b; simpl. contradiction. list_solve. apply wf_poly_nil. clear a0.
+    rewrite poly_mult_comm;try apply H3. symmetry. apply poly_add_id. all: assumption.
+  - unfold poly_div. destruct (poly_div_aux a b nil a Hb Ha). simpl. destruct x; simpl in *.
+    assert (deg p0 < deg b /\
+     wf_poly p /\ wf_poly p0 /\ (a = poly_add nil a -> a = poly_add (poly_mult b p) p0)).
+    apply a0. destruct b; simpl. contradiction. list_solve. apply wf_poly_nil. clear a0.
+    destruct H4. destruct H5. destruct H6.
+    assert (p = q /\ p0 = r). eapply remainder_unique. apply Ha. apply Hb. 
+    all: try assumption. rewrite poly_mult_comm; try assumption. apply H7.
+    symmetry. apply poly_add_id. assumption. destruct H8; subst. reflexivity.
+Qed.  
+    
+End DivFacts.
